theories/prelude/finitary.v
@@ -1,0 +1,207 @@
+From Coq.Unicode Require Import Utf8.
+From Coq.micromega Require Import Lia.
+From aneris.prelude Require Import classical quantifiers.
+From stdpp Require Import finite fin_sets.
+
+Section finite_smaller_card_nat.
+  Context {A} `{!EqDecision A}.
+
+  Fixpoint list_generated_by (f : nat → A) (n : nat) : list A :=
+    match n with
+    | O => [f 0]
+    | S n => f (S n) :: list_generated_by f n
+    end.
+
+  Lemma list_generated_by_length (f : nat → A) n :
+    length (list_generated_by f n) = S n.
+  Proof. induction n as [|? IHn]; [|simpl; rewrite IHn]; done. Qed.
+
+  Lemma elem_of_list_generated_by (f : nat → A) n x :
+    x ∈ list_generated_by f n ↔ ∃ m, m ≤ n ∧ x = f m.
+  Proof.
+    split.
+    - induction n; simpl.
+      + intros ->%elem_of_list_singleton; eauto.
+      + intros [->|Hn]%elem_of_cons; [by eauto|].
+        apply IHn in Hn as (?&?&?); eauto.
+    - intros [m [Hm1 ->]].
+      revert m Hm1; induction n; intros m Hm.
+      + replace m with 0 by lia.
+        apply elem_of_list_singleton; done.
+      + destruct (decide (m = S n)) as [->|].
+        * simpl; apply elem_of_cons; auto.
+        * simpl; apply elem_of_cons; auto with lia.
+  Qed.
+
+  Lemma list_generated_by_NoDup (f : nat → A) n :
+    injective f → NoDup (list_generated_by f n).
+  Proof.
+    intros Hf.
+    induction n; simpl.
+    - repeat constructor; set_solver.
+    - constructor; [|done].
+      intros (?&?&?%Hf)%elem_of_list_generated_by; lia.
+  Qed.
+
+  Lemma finite_smaller_card_nat : Finite A → smaller_card A nat.
+  Proof.
+    destruct 1 as [enum Henum Hin].
+    intros f Hf.
+    assert (length (list_generated_by f (length enum)) ≤ length enum) as Hlen.
+    { apply submseteq_length.
+      apply NoDup_submseteq; auto using list_generated_by_NoDup. }
+    rewrite list_generated_by_length in Hlen; lia.
+  Qed.
+
+End finite_smaller_card_nat.
+
+Definition surjective {A B} (f : A → B) := ∀ y, ∃ x, f x = y.
+
+Section smaller_card_nat_finite.
+  Context {A} `{!Inhabited A} `{!EqDecision A}.
+
+  Section no_surj_inj.
+    Context (Hnj : ∀ h : nat → A, ¬ surjective h).
+
+    Lemma nosurj_new_elem_exist (l : list A) : ∃ x, x ∉ l.
+    Proof.
+      specialize (Hnj (λ n, nth n l inhabitant)).
+      apply not_forall_exists_not in Hnj as [x Hx].
+      exists x.
+      intros [n Hn]%elem_of_list_lookup_1.
+      apply (nth_lookup_Some _ _ inhabitant) in Hn.
+      eapply not_exists_forall_not in Hx; eauto.
+    Qed.
+
+    Fixpoint nosurj_make_list (l : list A) (n : nat) : list A :=
+      match n with
+      | 0 => l
+      | S n' =>
+        nosurj_make_list l n' ++
+        [epsilon (nosurj_new_elem_exist (nosurj_make_list l n'))]
+      end.
+
+    Lemma nosurj_make_list_length l n :
+      length (nosurj_make_list l n) = length l + n.
+    Proof.
+      induction n as [|n IHn]; [simpl; lia|].
+      simpl; rewrite app_length, IHn; simpl; lia.
+    Qed.
+
+    Lemma nosurj_make_list_prefix l n1 n2 :
+      n1 ≤ n2 → (nosurj_make_list l n1) `prefix_of` (nosurj_make_list l n2).
+    Proof.
+      induction 1 as [|n2 IHn12]; [done|].
+      simpl; apply prefix_app_r; done.
+    Qed.
+
+    Lemma nosurj_make_list_NoDup l n : NoDup l → NoDup (nosurj_make_list l n).
+    Proof.
+      revert l; induction n; intros l Hl; [done|].
+      simpl.
+      apply NoDup_app; split; [auto; done|].
+      split; [|apply NoDup_singleton].
+      intros x Hx ->%elem_of_list_singleton.
+      apply (epsilon_correct _ (nosurj_new_elem_exist (nosurj_make_list l n)));
+        done.
+    Qed.
+
+    Definition nosurj_make_inj_fun (n : nat) : A :=
+      default inhabitant (nosurj_make_list [] (S n) !! n).
+
+    Lemma nosurj_make_inj_fun_inj : injective nosurj_make_inj_fun.
+    Proof.
+      assert (∀ n m, n ≤ m → nosurj_make_inj_fun n = nosurj_make_inj_fun m → n = m)
+        as Hnm.
+      { intros n m Hnm Hfnm.
+        unfold nosurj_make_inj_fun in Hfnm.
+        pose proof (lookup_lt_is_Some_2 (nosurj_make_list [] (S n)) n) as [k Hk].
+        { rewrite nosurj_make_list_length; lia. }
+        pose proof (lookup_lt_is_Some_2 (nosurj_make_list [] (S m)) m) as [l Hl].
+        { rewrite nosurj_make_list_length; lia. }
+        rewrite Hk, Hl in Hfnm; simpl in Hfnm; simplify_eq.
+        apply (NoDup_lookup (nosurj_make_list [] (S m)) n m l); [| |done].
+        - apply nosurj_make_list_NoDup, NoDup_nil_2.
+        - apply  (prefix_lookup
+                    (nosurj_make_list [] (S n)) (nosurj_make_list [] (S m)) n l);
+            [done|].
+          apply nosurj_make_list_prefix; lia.
+      }
+      intros n m.
+      destruct (decide (n < m)).
+      - apply Hnm; lia.
+      - intros; symmetry; apply Hnm; [lia|done].
+    Qed.
+
+  End no_surj_inj.
+
+  Definition least_domain_subset_including (h : nat → A) (x : A) : subset nat :=
+    λ k, ∀ n, (∃ m, m ≤ n ∧ h m = x) → k ≤ n.
+
+  Lemma least_domain_subset_including_all_not_cofinal (h : nat → A) :
+    surjective h → ∀ x, ¬ cofinal nat le (least_domain_subset_including h x).
+  Proof.
+    intros Hh x Hcf.
+    destruct (Hh x) as [k Hk].
+    destruct (Hcf (S k)) as [l [Hl1 Hl2]].
+    specialize (Hl1 k).
+    assert (l ≤ k); [eauto|lia].
+  Qed.
+
+  Lemma serjective_pre_image_bounded (h : nat → A) (Hhsurj : surjective h) :
+    smaller_card A nat → ∃ n, ∀ a, ∃ i, i ≤ n ∧ h i = a.
+  Proof.
+    intros Hsmc.
+    assert (¬ cofinal
+              nat le (quantifiers.union _ (least_domain_subset_including h)))
+      as Hncf.
+    { intros [x Hx]%regular_union_biger; auto using nat_regular with lia.
+      apply least_domain_subset_including_all_not_cofinal in Hx; done. }
+    apply not_forall_exists_not in Hncf as [n Hncf].
+    exists n; intros a.
+    destruct (dec_inh_nat_subset_has_unique_least_element (λ n, h n = a))
+      as [i [[Hi1 Hi2] Hi3]]; [|apply Hhsurj; done|].
+    { intros k; destruct (decide (h k = a)); eauto. }
+    exists i; split; [|done].
+    destruct (decide (i < n)); [lia|].
+    exfalso; apply Hncf.
+    exists i; split; [|lia].
+    exists a; intros m [j [Hj1 Hj2]].
+    etrans; [apply Hi2; apply Hj2|lia].
+  Qed.
+
+  Lemma smaller_card_nat_finite `{!EqDecision A} :
+    smaller_card A nat → Finite A.
+  Proof.
+    intros HA.
+    apply (epsilon (P := λ _, True)).
+    destruct (ExcludedMiddle (∃ h : nat → A, surjective h)) as [[h Hh]|Hnsurj].
+    - destruct (serjective_pre_image_bounded h) as [n Hn]; [done|done|].
+      unshelve eexists {| enum := remove_dups (list_generated_by h n) |};
+        [| |done].
+      + apply NoDup_remove_dups.
+      + intros a; apply elem_of_remove_dups.
+        destruct (Hn a) as [i [Hi1 Hi2]].
+        apply elem_of_list_generated_by; eauto.
+    - assert (∀ h : nat → A, ¬ surjective h) as Hnsurj'.
+      { apply not_exists_forall_not; done. }
+      specialize (HA (nosurj_make_inj_fun Hnsurj')).
+      exfalso; apply HA.
+      apply nosurj_make_inj_fun_inj.
+  Qed.
+
+End smaller_card_nat_finite.
+
+Section finite_lemmas.
+  Context `{!EqDecision A} `{!EqDecision B}.
+
+  Lemma sig_finite_and (P : A → Prop) (Q : B → Prop)
+        `{!∀ x, Decision (P x)} `{!∀ x, ProofIrrel (P x)}
+        `{!∀ x, Decision (Q x)} `{!∀ x, ProofIrrel (Q x)} :
+    Finite {x : A | P x} →
+    Finite {x : B | Q x} →
+    Finite {x : A * B | P (fst x) ∧ (Q (snd x))}.
+  Proof.
+  Admitted.
+
+End finite_lemmas.
